Fixed contradictory assumptions from TaggedGLS, and adjusted proof

ironfleet/src/Dafny/Distributed/Protocol/Lock/PerformanceProof/Definitions.i.dfy
@@ -1,49 +1,79 @@
 include "../../../Services/Lock/LockTaggedDistributedSystem.i.dfy"
-  include "TaggedGLS.i.dfy"
+  //include "TaggedGLS.i.dfy"
 
 module PerformanceProof__Definitions_i {
-import opened LockTaggedDistributedSystem_i
+ import opened LockTaggedDistributedSystem_i
   // import opened TaggedGLS_i
 
-function PerfBoundLockHeld(epoch: int) : PerfReport
+function PerfBoundLockHeld(epoch: int) : PerfExpr
   requires 0 < epoch
 {
-  var s : multiset<PerformanceReport> := multiset{};
-  var s2 := s[PerfStep(GrantStep) := epoch - 1][PerfStep(AcceptStep) := epoch - 1][PerfDelivery := epoch - 1];
-  PerfAdd(s2)
+    var s : multiset<PerfExpr> := multiset{};
+    var s2 := s[PerfStep(GrantStep) := epoch - 1][PerfStep(AcceptStep) := epoch - 1][PerfDelivery := epoch - 1];
+    PerfAdd(s2)
 }
 
-function PerfBoundLockInNetwork(epoch: int) : PerfReport
+function PerfBoundLockInNetwork(epoch: int) : PerfExpr
   requires 1 < epoch
 {
-  var s : multiset<PerformanceReport> := multiset{};
+  var s : multiset<PerfExpr> := multiset{};
   var s2 := s[PerfStep(GrantStep) := epoch - 1][PerfStep(AcceptStep) := epoch - 2][PerfDelivery := epoch - 2];
   PerfAdd(s2)
 }
 
+lemma Test(j:int)
+  requires 1 < j
+{
+  PerfProperties();
+  quotient_axioms();
+  var p := quotient_map(PerfVoid);
+  var p' := quotient_map(PerfBoundLockHeld(j));
+  var pkt_pr := quotient_map(PerfBoundLockInNetwork(j));
+
+  var deliveryTime := PerfAdd(pkt_pr, quotient_map(PerfDelivery));
+  var handlerStartTime := PerfMax(deliveryTime, p);
+  var totalTime := PerfAdd(handlerStartTime, quotient_map(PerfStep(AcceptStep)));
+
+  assert totalTime == p';
+}
+
+/*
 lemma {:verify false} specific_axiom(a:multiset<PerfExpr>, b:multiset<PerfExpr>)
   ensures PerfEq(PerfAdd(b + multiset{PerfAdd(a)}), PerfAdd(b + a))
 {
 }
 
-lemma Test(ios:seq<TaggedLIoOp<EndPoint, LockMessage>>, j:int)
-  requires 1 < j
+lemma Other(j:int, pkt_pr: PerfReport, nd_pr:PerfReport, final_pr:PerfReport)
+  requires 1 < j;
+  requires PerfEq(pkt_pr, PerfBoundLockInNetwork(j));
+  // requires PerfEq(nd_pr, PerfVoid);
+  requires nd_pr == PerfVoid;
+  ensures PerfEq(PerfAdd2(PerfMax(multiset{PerfAdd2(pkt_pr, PerfDelivery), nd_pr}), PerfStep(AcceptStep)), PerfBoundLockHeld(j));
+{
+  Test(j, pkt_pr, nd_pr, final_pr);
+}
+
+
+lemma Test(j:int, pkt_pr: PerfReport, nd_pr:PerfReport, final_pr:PerfReport)
+  requires 1 < j;
+  // requires PerfEq(pkt_pr, PerfBoundLockInNetwork(j));
+  requires pkt_pr == PerfBoundLockInNetwork(j);
+  // requires PerfEq(nd_pr, PerfVoid);
+  requires nd_pr == PerfVoid;
+  ensures PerfEq(PerfAdd2(PerfMax(multiset{PerfAdd2(pkt_pr, PerfDelivery), nd_pr}), PerfStep(AcceptStep)), PerfBoundLockHeld(j));
+
 {
   PerfProperties();
-  // var p := PerfBoundLockHeld(j)
-  // var p' := PerfBoundLockInNetwork(j + 1);
-
-  assume |ios| == 1 && ios[0].LIoOpReceive?;
-  assume PerfEq(ios[0].r.msg.pr, PerfBoundLockInNetwork(j));
-
-  var p := PerfVoid;
-  var p' := PerfBoundLockHeld(j);
-
-  var deliveryTime := PerfAdd2(ios[0].r.msg.pr, PerfDelivery);
-  var handlerStartTime := PerfMax(multiset{deliveryTime, p});
-  var totalTime := PerfAdd2(handlerStartTime, PerfStep(AcceptStep));
-
-  assert PerfEq(totalTime, p');
+// 
+  // var p := PerfVoid;
+  // var p' := PerfBoundLockHeld(j);
+  // // var pkt_pr := PerfBoundLockInNetwork(j);
+// 
+  // var deliveryTime := PerfAdd2(pkt_pr, PerfDelivery);
+  // var handlerStartTime := PerfMax(multiset{deliveryTime, p});
+  // var totalTime := PerfAdd2(handlerStartTime, PerfStep(AcceptStep));
+// 
+  // assert PerfEq(totalTime, p');
 }
 
 // if |ios| > 0 && ios[0].LIoOpReceive? then
@@ -54,5 +84,6 @@ lemma Test(ios:seq<TaggedLIoOp<EndPoint, LockMessage>>, j:int)
 // else
   // var totalTime := PerfAdd2(ios[0].pr, PerfStep(GrantStep));
 
+*/
   
 }
