ironfleet/src/Dafny/Distributed/Common/Framework/Performance.s.dfy
@@ -16,31 +16,47 @@ abstract module Performance_s {
 
   predicate {:axiom} PerfEq(p1:PerfExpr, p2:PerfExpr)
     ensures p1 == p2 ==> PerfEq(p1, p2)
-    ensures p1.PerfMax? && p1.prs == multiset{p2} ==> PerfEq(p1, p2)
-    ensures p1.PerfMax? && p1.prs == multiset{} && p2 == PerfZero() ==> PerfEq(p1, p2)
+    // ensures p1.PerfMax? && p1.prs == multiset{p2} ==> PerfEq(p1, p2)
+    // ensures p1.PerfMax? && p1.prs == multiset{} && p2 == PerfZero() ==> PerfEq(p1, p2)
 
-    ensures p1.PerfMax? && p2.PerfMax? && p2.prs == p1.prs - multiset{PerfVoid} ==> PerfEq(p1, p2)
+    // ensures p1.PerfMax? && p2.PerfMax? && p2.prs == p1.prs - multiset{PerfVoid} ==> PerfEq(p1, p2)
 
-    ensures p1.PerfAdd? && PerfVoid in p1.prs && p2 == PerfZero ==> PerfEq(p1, p2)
-    ensures p1.PerfAdd? && p2 == PerfAdd(p1.prs[PerfZero() := 0]) ==> PerfEq(p1, p2)
-    ensures p1.PerfAdd? && p1.prs == multiset{} && p2 == PerfZero ==> PerfEq(p1, p2)
-    ensures p2.PerfAdd? && p2.prs == multiset{} && p1 == PerfZero ==> PerfEq(p1, p2)
+    // ensures p1.PerfAdd? && PerfVoid in p1.prs && p2 == PerfZero ==> PerfEq(p1, p2)
+    // ensures p1.PerfAdd? && p2 == PerfAdd(p1.prs[PerfZero() := 0]) ==> PerfEq(p1, p2)
+    // ensures p1.PerfAdd? && p1.prs == multiset{} && p2 == PerfZero ==> PerfEq(p1, p2)
+    // ensures p2.PerfAdd? && p2.prs == multiset{} && p1 == PerfZero ==> PerfEq(p1, p2)
 
     // Want to establish associativity
     // PerfAdd(multiset{PerfAdd(p1), prs'}) == PerfAdd(p1 + prs')
     // ensures forall prs :: p1.PerfAdd? && PerfAdd(prs) in p1.prs && p2 == PerfAdd(p1.prs + prs - multiset{PerfAdd(prs)}) ==> PerfEq(p1, p2)
     // ensures p1.PerfAdd? ==> (forall pr :: pr in p1.prs && pr.PerfAdd? && p2 == PerfAdd(p1.prs + pr.prs - multiset{PerfAdd(pr.prs)}) ==> PerfEq(p1, p2))
 
-    predicate {:axiom} PerfLe(p1: PerfExpr, p2:PerfExpr)
+  lemma {:axiom} PerfEq_IsEquivRelation()
+    ensures forall p1, p2 :: PerfEq(p1, p2) == PerfEq(p2, p1);
+    ensures forall p1, p2 :: p1 == p2 ==> PerfEq(p1, p2);
+    ensures forall p1, p2, p3 :: PerfEq(p1, p2) && PerfEq(p2, p3) ==> PerfEq(p1, p3);
+
+  lemma {:axiom} PerfAdd_IsAssociative()
 
   lemma {:axiom} PerfProperties()
+    // PerfLe is a partial order
+    // ensures forall p1, p2 :: PerfEq(p1, p2) ==> PerfLe(p1, p2) && PerfLe(p2, p1);
+    // ensures forall p1, p2, p3 :: PerfLe(p1, p2) && PerfLe(p2, p3) ==> PerfLe(p1, p3);
+
+    // 
+    // ensures forall p1, p2, p1', p2' :: PerfEq(p1, p1') && PerfEq(p2, p2') ==> PerfLe(p1, p2) == PerfLe(p1', p2')
+
+    // PerfMax is bigger than all prs
+    // ensures forall prs {:trigger PerfMax(prs)} :: (forall pr :: pr in prs ==> PerfLe(pr, PerfMax(prs)));
+
     // PerfEq is a equivalence relation
     ensures forall p1, p2 :: PerfEq(p1, p2) == PerfEq(p2, p1);
     ensures forall p1, p2 :: p1 == p2 ==> PerfEq(p1, p2);
     ensures forall p1, p2, p3 :: PerfEq(p1, p2) && PerfEq(p2, p3) ==> PerfEq(p1, p3);
 
-    // axioms involving PerfEq
-    ensures forall p1, p2, p3 :: PerfEq(PerfAdd2(p1, PerfAdd2(p2, p3)), PerfAdd(multiset{p1, p2, p3}));
+    // axioms involving PerfAdd
+    ensures forall p1:PerfExpr, p2 :: p1.PerfAdd? && p1.prs == multiset{} && p2 == PerfZero ==> PerfEq(p1, p2)
+    ensures forall p1, p2, p3 {:trigger PerfAdd2(p1, PerfAdd2(p2, p3))} :: PerfEq(PerfAdd2(p1, PerfAdd2(p2, p3)), PerfAdd(multiset{p1, p2, p3}));
     ensures forall p1, p2 :: (forall p1' :: PerfEq(p1, p1') ==> PerfEq(PerfAdd2(p1, p2), PerfAdd2(p1', p2)));
     ensures forall p1, p2, p1', p2' :: PerfEq(p1, p1') && PerfEq(p2, p2') ==> PerfEq(PerfAdd2(p1, p2), PerfAdd2(p1', p2'));
 
