ironfleet/src/Dafny/Distributed/Protocol/Lock/PerformanceProof/TaggedGLS.i.dfy
@@ -50,20 +50,15 @@ datatype TaggedGLS_State = TaggedGLS_State(
     LS_NextOneServer(UntagLS_State(tls), UntagLS_State(tls'), id, UntagLIoOpSeq(ios), hstep)
       && (
       if |ios| > 0 && ios[0].LIoOpReceive? then
-      (var deliveryTime := PerfAdd2(ios[0].r.msg.pr, PerfDelivery);
-      var handlerStartTime := PerfMax(multiset{deliveryTime, tls.t_servers[id].pr});
-      var totalTime := PerfAdd2(handlerStartTime, PerfStep(GrantStep));
-      totalTime == tls'.t_servers[id].pr)
+        var deliveryTime := PerfAdd2(ios[0].r.msg.pr, PerfDelivery);
+        var handlerStartTime := PerfMax(multiset{deliveryTime, tls.t_servers[id].pr});
+        var totalTime := PerfAdd2(handlerStartTime, PerfStep(hstep));
+        totalTime == tls'.t_servers[id].pr
       else
-        var totalTime := PerfAdd2(tls.t_servers[id].pr, PerfStep(GrantStep));
+        var totalTime := PerfAdd2(tls.t_servers[id].pr, PerfStep(hstep));
         totalTime == tls'.t_servers[id].pr
       )
 
-      && (var deliveryTime := PerfMax(multiset(GetReceivePRs(ios)));
-      var recvTime := PerfAdd2(deliveryTime, PerfDelivery);
-      var totalTime := PerfAdd2(recvTime, PerfStep(hstep));
-      tls'.t_servers[id].pr == totalTime
-      )
       && (forall t_io :: t_io in ios && t_io.LIoOpSend? ==> t_io.s.msg.pr == tls'.t_servers[id].pr)
       && tls'.t_servers == tls.t_servers[id := tls'.t_servers[id]]
   }
